DynamoDbEncryption/runtimes/go/ImplementationFromDafny-go/awscryptographydbencryptionsdkdynamodbsmithygeneratedtypes/types.go
@@ -546,6 +546,9 @@ func (input StandardBeacon) Validate() error {
 		if *input.NumberOfBuckets < 1 {
 			return fmt.Errorf("BucketCount has a minimum of 1 but has the value of %d.", *input.NumberOfBuckets)
 		}
+		if *input.NumberOfBuckets > 255 {
+			return fmt.Errorf("BucketCount has a maximum of 255 but has the value of %d.", *input.NumberOfBuckets)
+		}
 	}
 	if input.Aws_cryptography_dbEncryptionSdk_dynamoDb_StandardBeacon_style_Validate() != nil {
 		return input.Aws_cryptography_dbEncryptionSdk_dynamoDb_StandardBeacon_style_Validate()
@@ -832,6 +835,9 @@ func (input BeaconVersion) Validate() error {
 		if *input.NumberOfBuckets < 1 {
 			return fmt.Errorf("BucketCount has a minimum of 1 but has the value of %d.", *input.NumberOfBuckets)
 		}
+		if *input.NumberOfBuckets > 255 {
+			return fmt.Errorf("BucketCount has a maximum of 255 but has the value of %d.", *input.NumberOfBuckets)
+		}
 	}
 	if len(input.SignedParts) < 1 {
 		return fmt.Errorf("SignedPartsList has a minimum length of 1 but has the length of %d.", len(input.SignedParts))
@@ -911,6 +917,29 @@ func (input BeaconVersion) Aws_cryptography_dbEncryptionSdk_dynamoDb_BeaconVersi
 			return item.Validate()
 		}
 	}
+
+	return nil
+}
+
+type GetBucketNumberOutput struct {
+	BucketNumber int32
+}
+
+func (input GetBucketNumberOutput) Validate() error {
+	if input.BucketNumber < 0 {
+		return fmt.Errorf("BucketNumber has a minimum of 0 but has the value of %d.", input.BucketNumber)
+	}
+	if input.BucketNumber > 254 {
+		return fmt.Errorf("BucketNumber has a maximum of 254 but has the value of %d.", input.BucketNumber)
+	}
+
+	return nil
+}
+
+type BucketSelectorReference struct {
+}
+
+func (input BucketSelectorReference) Validate() error {
 
 	return nil
 }
@@ -1022,6 +1051,8 @@ type DynamoDbTableEncryptionConfig struct {
 	AllowedUnsignedAttributePrefix *string
 
 	AllowedUnsignedAttributes []string
+
+	BucketSelector IBucketSelector
 
 	Cmm awscryptographymaterialproviderssmithygeneratedtypes.ICryptographicMaterialsManager
 
@@ -1262,6 +1293,141 @@ func (input GetBranchKeyIdFromDdbKeyInput) Aws_cryptography_dbEncryptionSdk_dyna
 	return nil
 }
 
+type GetBucketNumberInput struct {
+	Item map[string]dynamodbtypes.AttributeValue
+
+	NumberOfBuckets int32
+}
+
+func (input GetBucketNumberInput) Validate() error {
+	if input.Item == nil {
+		return fmt.Errorf("input.Item is required but has a nil value.")
+	}
+	if input.Aws_cryptography_dbEncryptionSdk_dynamoDb_GetBucketNumberInput_item_Validate() != nil {
+		return input.Aws_cryptography_dbEncryptionSdk_dynamoDb_GetBucketNumberInput_item_Validate()
+	}
+	if input.NumberOfBuckets < 1 {
+		return fmt.Errorf("BucketCount has a minimum of 1 but has the value of %d.", input.NumberOfBuckets)
+	}
+	if input.NumberOfBuckets > 255 {
+		return fmt.Errorf("BucketCount has a maximum of 255 but has the value of %d.", input.NumberOfBuckets)
+	}
+
+	return nil
+}
+
+func (input GetBucketNumberInput) Com_amazonaws_dynamodb_AttributeMap_value_Validate(Value dynamodbtypes.AttributeValue) error {
+	if Value == nil {
+		return nil
+	}
+	switch unionType := Value.(type) {
+	case *dynamodbtypes.AttributeValueMemberS:
+	case *dynamodbtypes.AttributeValueMemberN:
+	case *dynamodbtypes.AttributeValueMemberB:
+	case *dynamodbtypes.AttributeValueMemberSS:
+	case *dynamodbtypes.AttributeValueMemberNS:
+	case *dynamodbtypes.AttributeValueMemberBS:
+	case *dynamodbtypes.AttributeValueMemberM:
+	case *dynamodbtypes.AttributeValueMemberL:
+	case *dynamodbtypes.AttributeValueMemberNULL:
+	case *dynamodbtypes.AttributeValueMemberBOOL:
+	// Default case should not be reached.
+	default:
+		panic(fmt.Sprintf("Unhandled union type: %T ", unionType))
+	}
+
+	return nil
+}
+func (input GetBucketNumberInput) Com_amazonaws_dynamodb_MapAttributeValue_value_Validate(Value dynamodbtypes.AttributeValue) error {
+	if Value == nil {
+		return nil
+	}
+	switch unionType := Value.(type) {
+	case *dynamodbtypes.AttributeValueMemberS:
+	case *dynamodbtypes.AttributeValueMemberN:
+	case *dynamodbtypes.AttributeValueMemberB:
+	case *dynamodbtypes.AttributeValueMemberSS:
+	case *dynamodbtypes.AttributeValueMemberNS:
+	case *dynamodbtypes.AttributeValueMemberBS:
+	case *dynamodbtypes.AttributeValueMemberM:
+		if input.Com_amazonaws_dynamodb_AttributeValue_M_Validate(unionType.Value) != nil {
+			return input.Com_amazonaws_dynamodb_AttributeValue_M_Validate(unionType.Value)
+		}
+	case *dynamodbtypes.AttributeValueMemberL:
+	case *dynamodbtypes.AttributeValueMemberNULL:
+	case *dynamodbtypes.AttributeValueMemberBOOL:
+	// Default case should not be reached.
+	default:
+		panic(fmt.Sprintf("Unhandled union type: %T ", unionType))
+	}
+
+	return nil
+}
+func (input GetBucketNumberInput) Com_amazonaws_dynamodb_AttributeValue_M_Validate(Value map[string]dynamodbtypes.AttributeValue) error {
+	for key, value := range Value {
+		if len(key) < 0 {
+			return fmt.Errorf("AttributeName has a minimum length of 0 but has the length of %d.", len(key))
+		}
+		if len(key) > 65535 {
+			return fmt.Errorf("AttributeName has a maximum length of 65535 but has the length of %d.", len(key))
+		}
+		if input.Com_amazonaws_dynamodb_MapAttributeValue_value_Validate(value) != nil {
+			return input.Com_amazonaws_dynamodb_MapAttributeValue_value_Validate(value)
+		}
+	}
+
+	return nil
+}
+func (input GetBucketNumberInput) Com_amazonaws_dynamodb_ListAttributeValue_member_Validate(Value dynamodbtypes.AttributeValue) error {
+	if Value == nil {
+		return nil
+	}
+	switch unionType := Value.(type) {
+	case *dynamodbtypes.AttributeValueMemberS:
+	case *dynamodbtypes.AttributeValueMemberN:
+	case *dynamodbtypes.AttributeValueMemberB:
+	case *dynamodbtypes.AttributeValueMemberSS:
+	case *dynamodbtypes.AttributeValueMemberNS:
+	case *dynamodbtypes.AttributeValueMemberBS:
+	case *dynamodbtypes.AttributeValueMemberM:
+	case *dynamodbtypes.AttributeValueMemberL:
+		if input.Com_amazonaws_dynamodb_AttributeValue_L_Validate(unionType.Value) != nil {
+			return input.Com_amazonaws_dynamodb_AttributeValue_L_Validate(unionType.Value)
+		}
+	case *dynamodbtypes.AttributeValueMemberNULL:
+	case *dynamodbtypes.AttributeValueMemberBOOL:
+	// Default case should not be reached.
+	default:
+		panic(fmt.Sprintf("Unhandled union type: %T ", unionType))
+	}
+
+	return nil
+}
+func (input GetBucketNumberInput) Com_amazonaws_dynamodb_AttributeValue_L_Validate(Value []dynamodbtypes.AttributeValue) error {
+	for _, item := range Value {
+		if input.Com_amazonaws_dynamodb_ListAttributeValue_member_Validate(item) != nil {
+			return input.Com_amazonaws_dynamodb_ListAttributeValue_member_Validate(item)
+		}
+	}
+
+	return nil
+}
+func (input GetBucketNumberInput) Aws_cryptography_dbEncryptionSdk_dynamoDb_GetBucketNumberInput_item_Validate() error {
+	for key, value := range input.Item {
+		if len(key) < 0 {
+			return fmt.Errorf("AttributeName has a minimum length of 0 but has the length of %d.", len(key))
+		}
+		if len(key) > 65535 {
+			return fmt.Errorf("AttributeName has a maximum length of 65535 but has the length of %d.", len(key))
+		}
+		if input.Com_amazonaws_dynamodb_AttributeMap_value_Validate(value) != nil {
+			return input.Com_amazonaws_dynamodb_AttributeMap_value_Validate(value)
+		}
+	}
+
+	return nil
+}
+
 // BeaconKeySourceMembermulti
 // BeaconKeySourceMembersingle
 type BeaconKeySource interface {
@@ -1395,6 +1561,10 @@ type DynamoDbEncryptionBaseException interface {
 	// aren't useful for type assertion checks. No concrete class is expected to implement
 	// this method. This is also not exported.
 	interfaceBindingMethod()
+}
+
+type IBucketSelector interface {
+	GetBucketNumber(GetBucketNumberInput) (*GetBucketNumberOutput, error)
 }
 
 type IDynamoDbKeyBranchKeyIdSupplier interface {
