DynamoDbEncryption/runtimes/java/src/main/smithy-generated/software/amazon/cryptography/dbencryptionsdk/dynamodb/model/DynamoDbTableEncryptionConfig.java
@@ -6,6 +6,8 @@ package software.amazon.cryptography.dbencryptionsdk.dynamodb.model;
 import java.util.List;
 import java.util.Map;
 import java.util.Objects;
+import software.amazon.cryptography.dbencryptionsdk.dynamodb.BucketSelector;
+import software.amazon.cryptography.dbencryptionsdk.dynamodb.IBucketSelector;
 import software.amazon.cryptography.dbencryptionsdk.structuredencryption.model.CryptoAction;
 import software.amazon.cryptography.materialproviders.CryptographicMaterialsManager;
 import software.amazon.cryptography.materialproviders.ICryptographicMaterialsManager;
@@ -78,6 +80,11 @@ public class DynamoDbTableEncryptionConfig {
    */
   private final PlaintextOverride plaintextOverride;
 
+  /**
+   * How to choose the bucket for an item. Default behavior is a random between 0 and numberOfBuckets.
+   */
+  private final IBucketSelector bucketSelector;
+
   protected DynamoDbTableEncryptionConfig(BuilderImpl builder) {
     this.logicalTableName = builder.logicalTableName();
     this.partitionKeyName = builder.partitionKeyName();
@@ -92,6 +99,7 @@ public class DynamoDbTableEncryptionConfig {
     this.cmm = builder.cmm();
     this.legacyOverride = builder.legacyOverride();
     this.plaintextOverride = builder.plaintextOverride();
+    this.bucketSelector = builder.bucketSelector();
   }
 
   /**
@@ -176,6 +184,13 @@ public class DynamoDbTableEncryptionConfig {
    */
   public PlaintextOverride plaintextOverride() {
     return this.plaintextOverride;
+  }
+
+  /**
+   * @return How to choose the bucket for an item. Default behavior is a random between 0 and numberOfBuckets.
+   */
+  public IBucketSelector bucketSelector() {
+    return this.bucketSelector;
   }
 
   public Builder toBuilder() {
@@ -311,6 +326,16 @@ public class DynamoDbTableEncryptionConfig {
      */
     PlaintextOverride plaintextOverride();
 
+    /**
+     * @param bucketSelector How to choose the bucket for an item. Default behavior is a random between 0 and numberOfBuckets.
+     */
+    Builder bucketSelector(IBucketSelector bucketSelector);
+
+    /**
+     * @return How to choose the bucket for an item. Default behavior is a random between 0 and numberOfBuckets.
+     */
+    IBucketSelector bucketSelector();
+
     DynamoDbTableEncryptionConfig build();
   }
 
@@ -340,6 +365,8 @@ public class DynamoDbTableEncryptionConfig {
 
     protected PlaintextOverride plaintextOverride;
 
+    protected IBucketSelector bucketSelector;
+
     protected BuilderImpl() {}
 
     protected BuilderImpl(DynamoDbTableEncryptionConfig model) {
@@ -356,6 +383,7 @@ public class DynamoDbTableEncryptionConfig {
       this.cmm = model.cmm();
       this.legacyOverride = model.legacyOverride();
       this.plaintextOverride = model.plaintextOverride();
+      this.bucketSelector = model.bucketSelector();
     }
 
     public Builder logicalTableName(String logicalTableName) {
@@ -470,6 +498,15 @@ public class DynamoDbTableEncryptionConfig {
 
     public PlaintextOverride plaintextOverride() {
       return this.plaintextOverride;
+    }
+
+    public Builder bucketSelector(IBucketSelector bucketSelector) {
+      this.bucketSelector = BucketSelector.wrap(bucketSelector);
+      return this;
+    }
+
+    public IBucketSelector bucketSelector() {
+      return this.bucketSelector;
     }
 
     public DynamoDbTableEncryptionConfig build() {
