DynamoDbEncryption/runtimes/java/src/main/smithy-generated/software/amazon/cryptography/dbencryptionsdk/dynamodb/model/GetBucketNumberInput.java
@@ -1,0 +1,108 @@
+// Copyright Amazon.com Inc. or its affiliates. All Rights Reserved.
+// SPDX-License-Identifier: Apache-2.0
+// Do not modify this file. This file is machine generated, and any changes to it will be overwritten.
+package software.amazon.cryptography.dbencryptionsdk.dynamodb.model;
+
+import java.util.Map;
+import java.util.Objects;
+import software.amazon.awssdk.services.dynamodb.model.AttributeValue;
+
+public class GetBucketNumberInput {
+
+  private final Map<String, AttributeValue> item;
+
+  private final int numberOfBuckets;
+
+  protected GetBucketNumberInput(BuilderImpl builder) {
+    this.item = builder.item();
+    this.numberOfBuckets = builder.numberOfBuckets();
+  }
+
+  public Map<String, AttributeValue> item() {
+    return this.item;
+  }
+
+  public int numberOfBuckets() {
+    return this.numberOfBuckets;
+  }
+
+  public Builder toBuilder() {
+    return new BuilderImpl(this);
+  }
+
+  public static Builder builder() {
+    return new BuilderImpl();
+  }
+
+  public interface Builder {
+    Builder item(Map<String, AttributeValue> item);
+
+    Map<String, AttributeValue> item();
+
+    Builder numberOfBuckets(int numberOfBuckets);
+
+    int numberOfBuckets();
+
+    GetBucketNumberInput build();
+  }
+
+  static class BuilderImpl implements Builder {
+
+    protected Map<String, AttributeValue> item;
+
+    protected int numberOfBuckets;
+
+    private boolean _numberOfBucketsSet = false;
+
+    protected BuilderImpl() {}
+
+    protected BuilderImpl(GetBucketNumberInput model) {
+      this.item = model.item();
+      this.numberOfBuckets = model.numberOfBuckets();
+      this._numberOfBucketsSet = true;
+    }
+
+    public Builder item(Map<String, AttributeValue> item) {
+      this.item = item;
+      return this;
+    }
+
+    public Map<String, AttributeValue> item() {
+      return this.item;
+    }
+
+    public Builder numberOfBuckets(int numberOfBuckets) {
+      this.numberOfBuckets = numberOfBuckets;
+      this._numberOfBucketsSet = true;
+      return this;
+    }
+
+    public int numberOfBuckets() {
+      return this.numberOfBuckets;
+    }
+
+    public GetBucketNumberInput build() {
+      if (Objects.isNull(this.item())) {
+        throw new IllegalArgumentException(
+          "Missing value for required field `item`"
+        );
+      }
+      if (!this._numberOfBucketsSet) {
+        throw new IllegalArgumentException(
+          "Missing value for required field `numberOfBuckets`"
+        );
+      }
+      if (this._numberOfBucketsSet && this.numberOfBuckets() < 1) {
+        throw new IllegalArgumentException(
+          "`numberOfBuckets` must be greater than or equal to 1"
+        );
+      }
+      if (this._numberOfBucketsSet && this.numberOfBuckets() > 255) {
+        throw new IllegalArgumentException(
+          "`numberOfBuckets` must be less than or equal to 255."
+        );
+      }
+      return new GetBucketNumberInput(this);
+    }
+  }
+}
