DynamoDbEncryption/runtimes/java/src/main/smithy-generated/software/amazon/cryptography/dbencryptionsdk/dynamodb/model/GetBucketNumberOutput.java
@@ -1,0 +1,76 @@
+// Copyright Amazon.com Inc. or its affiliates. All Rights Reserved.
+// SPDX-License-Identifier: Apache-2.0
+// Do not modify this file. This file is machine generated, and any changes to it will be overwritten.
+package software.amazon.cryptography.dbencryptionsdk.dynamodb.model;
+
+public class GetBucketNumberOutput {
+
+  private final int bucketNumber;
+
+  protected GetBucketNumberOutput(BuilderImpl builder) {
+    this.bucketNumber = builder.bucketNumber();
+  }
+
+  public int bucketNumber() {
+    return this.bucketNumber;
+  }
+
+  public Builder toBuilder() {
+    return new BuilderImpl(this);
+  }
+
+  public static Builder builder() {
+    return new BuilderImpl();
+  }
+
+  public interface Builder {
+    Builder bucketNumber(int bucketNumber);
+
+    int bucketNumber();
+
+    GetBucketNumberOutput build();
+  }
+
+  static class BuilderImpl implements Builder {
+
+    protected int bucketNumber;
+
+    private boolean _bucketNumberSet = false;
+
+    protected BuilderImpl() {}
+
+    protected BuilderImpl(GetBucketNumberOutput model) {
+      this.bucketNumber = model.bucketNumber();
+      this._bucketNumberSet = true;
+    }
+
+    public Builder bucketNumber(int bucketNumber) {
+      this.bucketNumber = bucketNumber;
+      this._bucketNumberSet = true;
+      return this;
+    }
+
+    public int bucketNumber() {
+      return this.bucketNumber;
+    }
+
+    public GetBucketNumberOutput build() {
+      if (!this._bucketNumberSet) {
+        throw new IllegalArgumentException(
+          "Missing value for required field `bucketNumber`"
+        );
+      }
+      if (this._bucketNumberSet && this.bucketNumber() < 0) {
+        throw new IllegalArgumentException(
+          "`bucketNumber` must be greater than or equal to 0"
+        );
+      }
+      if (this._bucketNumberSet && this.bucketNumber() > 254) {
+        throw new IllegalArgumentException(
+          "`bucketNumber` must be less than or equal to 254."
+        );
+      }
+      return new GetBucketNumberOutput(this);
+    }
+  }
+}
