DynamoDbEncryption/runtimes/net/Generated/DynamoDbEncryption/BucketSelector.cs
@@ -1,0 +1,23 @@
+// Copyright Amazon.com Inc. or its affiliates. All Rights Reserved.
+// SPDX-License-Identifier: Apache-2.0
+// Do not modify this file. This file is machine generated, and any changes to it will be overwritten.
+using System;
+using System.IO;
+using System.Collections.Generic;
+using AWS.Cryptography.DbEncryptionSDK.DynamoDb;
+using software.amazon.cryptography.dbencryptionsdk.dynamodb.internaldafny.types;
+namespace AWS.Cryptography.DbEncryptionSDK.DynamoDb
+{
+  internal class BucketSelector : BucketSelectorBase
+  {
+    internal readonly software.amazon.cryptography.dbencryptionsdk.dynamodb.internaldafny.types.IBucketSelector _impl;
+    internal BucketSelector(software.amazon.cryptography.dbencryptionsdk.dynamodb.internaldafny.types.IBucketSelector impl) { this._impl = impl; }
+    protected override AWS.Cryptography.DbEncryptionSDK.DynamoDb.GetBucketNumberOutput _GetBucketNumber(AWS.Cryptography.DbEncryptionSDK.DynamoDb.GetBucketNumberInput input)
+    {
+      software.amazon.cryptography.dbencryptionsdk.dynamodb.internaldafny.types._IGetBucketNumberInput internalInput = TypeConversion.ToDafny_N3_aws__N12_cryptography__N15_dbEncryptionSdk__N8_dynamoDb__S20_GetBucketNumberInput(input);
+      Wrappers_Compile._IResult<software.amazon.cryptography.dbencryptionsdk.dynamodb.internaldafny.types._IGetBucketNumberOutput, software.amazon.cryptography.dbencryptionsdk.dynamodb.internaldafny.types._IError> result = this._impl.GetBucketNumber(internalInput);
+      if (result.is_Failure) throw TypeConversion.FromDafny_CommonError(result.dtor_error);
+      return TypeConversion.FromDafny_N3_aws__N12_cryptography__N15_dbEncryptionSdk__N8_dynamoDb__S21_GetBucketNumberOutput(result.dtor_value);
+    }
+  }
+}
