DynamoDbEncryption/runtimes/net/Generated/DynamoDbEncryption/BucketSelectorBase.cs
@@ -1,0 +1,16 @@
+// Copyright Amazon.com Inc. or its affiliates. All Rights Reserved.
+// SPDX-License-Identifier: Apache-2.0
+// Do not modify this file. This file is machine generated, and any changes to it will be overwritten.
+using System;
+using AWS.Cryptography.DbEncryptionSDK.DynamoDb;
+namespace AWS.Cryptography.DbEncryptionSDK.DynamoDb
+{
+  public abstract class BucketSelectorBase : IBucketSelector
+  {
+    public AWS.Cryptography.DbEncryptionSDK.DynamoDb.GetBucketNumberOutput GetBucketNumber(AWS.Cryptography.DbEncryptionSDK.DynamoDb.GetBucketNumberInput input)
+    {
+      input.Validate(); return _GetBucketNumber(input);
+    }
+    protected abstract AWS.Cryptography.DbEncryptionSDK.DynamoDb.GetBucketNumberOutput _GetBucketNumber(AWS.Cryptography.DbEncryptionSDK.DynamoDb.GetBucketNumberInput input);
+  }
+}
