DynamoDbEncryption/runtimes/net/Generated/DynamoDbEncryption/GetBucketNumberOutput.cs
@@ -1,0 +1,26 @@
+// Copyright Amazon.com Inc. or its affiliates. All Rights Reserved.
+// SPDX-License-Identifier: Apache-2.0
+// Do not modify this file. This file is machine generated, and any changes to it will be overwritten.
+using System;
+using AWS.Cryptography.DbEncryptionSDK.DynamoDb;
+namespace AWS.Cryptography.DbEncryptionSDK.DynamoDb
+{
+  public class GetBucketNumberOutput
+  {
+    private int? _bucketNumber;
+    public int BucketNumber
+    {
+      get { return this._bucketNumber.GetValueOrDefault(); }
+      set { this._bucketNumber = value; }
+    }
+    public bool IsSetBucketNumber()
+    {
+      return this._bucketNumber.HasValue;
+    }
+    public void Validate()
+    {
+      if (!IsSetBucketNumber()) throw new System.ArgumentException("Missing value for required property 'BucketNumber'");
+
+    }
+  }
+}
