DynamoDbEncryption/runtimes/net/Generated/DynamoDbEncryption/IBucketSelector.cs
@@ -1,0 +1,12 @@
+// Copyright Amazon.com Inc. or its affiliates. All Rights Reserved.
+// SPDX-License-Identifier: Apache-2.0
+// Do not modify this file. This file is machine generated, and any changes to it will be overwritten.
+using System;
+using AWS.Cryptography.DbEncryptionSDK.DynamoDb;
+namespace AWS.Cryptography.DbEncryptionSDK.DynamoDb
+{
+  public interface IBucketSelector
+  {
+    AWS.Cryptography.DbEncryptionSDK.DynamoDb.GetBucketNumberOutput GetBucketNumber(AWS.Cryptography.DbEncryptionSDK.DynamoDb.GetBucketNumberInput input);
+  }
+}
